2025-01-09 13:09
Status: 
Tags: [[First Theorems and Notation in Alg 1]] [[a to the n group theorem]]
# (a^m)n equals a^mn

TD: YEAR1::TERM1::MA151 Algebra 1::04 First Theorems and Notation
Q: Let $G$ be a group, and let $a âˆˆ G$ then prove $(a^{m})^{n}=a^{mn}$
A: If $m$ and $n$ are positive integers then $$ (a^m)^n = \underbrace{a a \cdots a}_{m \text{ times}} \underbrace{a a \cdots a}_{m \text{ times}} \cdots \underbrace{a a \cdots a}_{m \text{ times}} \quad \text{($n$ times)}. $$ From this it can be seen that $(a^m)^n = a^{mn}$. If $m$ is positive and $n$ is negative then we have $$ (a^m)^n = ((a^m)^{-n})^{-1} = (a^{-mn})^{-1} = ((a^{mn})^{-1})^{-1} = a^{mn} $$ using what we have just proved for positive integers and ii)
The other cases ($m$ negative and $n$ positive and $m$ and $n$ both negative are similar).
<!--ID: 1736428508639-->
