2025-01-15 08:36
Status: 
Tags: [[First Theorems and Notation in Alg 1]]
# abelian (ab)^n equals a^nb^n

TD: YEAR1::TERM1::MA151 Algebra 1::04 First Theorems and Notation
Q: Prove that if $G$ is abelian, $a, b âˆˆ G$ and $n$ an integer then $(ab)^n = a^ n b^ n$ .
A: Suppose $n$ is positive and $G$ is abelian.
Then$$
(ab)^n = \underbrace{ab \cdots ab}_{n \text{ times}} = \underbrace{aa \cdots a}_{n \text{ times}} \underbrace{bb \cdots b}_{n \text{ times}} = a^n b^n.
$$Note that the expressions either side of the second equals sign are the same only because $G$ is abelian.
Then, if $n$ is negative, we have$$
(ab)^n = ((ab)^{-n})^{-1} = ((ab)^{-1})^{-n} = (b^{-1} a^{-1})^{-n} = (b^{-1})^{-n} (a^{-1})^{-n} = b^n a^n = a^n b^n.
$$
<!--ID: 1736930287315-->

