2025-01-08 11:08
Status: 
Tags: [[First Theorems and Notation in Alg 1]] [[Group inverse existence]]
# inverse of ab

TD: YEAR1::TERM1::MA151 Algebra 1::04 First Theorems and Notation
Q: Let $G$ be a group and $a,b\in G$, then prove that $(ab)^{-1}=b^{-1}a^{-1}$
?
A:We are being asked to prove that $b^{-1}a^{-1}$ is the inverse of $ab$, so we WTS that $(b^{-1}a^{-1})(ab)=1=(ab)(b^{-1}a^{-1})$,
by associativity we can show that$$
\begin{align}
(b^{-1}a^{-1})(ab)&=b^{-1}(a^{-1}a)b\\
&=b^{-1}1b \\
&=1
\end{align}
$$ and similarly $(ab)(b^{-1}a^{-1})=1$.
<!--ID: 1736341416809-->
