{{date}} {{time}}
Status: 
Tags: [[Taylor's Theorem]]
# {{title}}

TD: YEAR1::TERM2::MA139 Analysis 2::04 Taylor's Theorem
Q: Proof for Taylor's Theorem Lagrange remainder using $g(x)$
A: The function $g$ given by $g(x)=$$$f(x) - \left( f(a) + f'(a)(x - a) + \cdots + \frac{f^{(n-1)}(a)}{(n - 1)!}(x - a)^{n-1} \right) $$satisfies $g(a) = 0$, $g'(a) = 0$, and so on up to $g^{(n-1)}(a) = 0$. It also satisfies $g^{(n)}(x) = f^{(n)}(x)$ for all $x$ because $f$ and $g$ differ by a polynomial of degree only $n - 1$.